src/lib/kuiper/Kuiper.Approximates.F64.fsti
@@ -1,0 +1,6 @@
+module Kuiper.Approximates.F64
+
+open Kuiper
+open Kuiper.Approximates.Class
+
+instance val real_like_f64 : real_like f64
