src/lib/kuiper/Kuiper.Approximates.U8.fst
@@ -1,0 +1,47 @@
+module Kuiper.Approximates.U8
+
+open Kuiper
+open Kuiper.Scalars
+open Kuiper.Approximates.Class
+open FStar.Real
+open Kuiper.Math.Silly { mod_prod }
+
+(* For the integer types, we can actually define the relation
+and prove it. BUT, we must consider overflow! So we make the relation
+weaker than you may expect. *)
+instance real_like_u8 : real_like u8 = {
+  to_real = (fun x -> Real.of_int (UInt8.v x));
+
+  approximates = (fun x r ->
+    exists (x' : int).
+      r == Real.of_int x' /\ UInt8.v x == x' % 256);
+
+  to_real_ok = (fun x -> ());
+
+  a0 = ();
+  a1 = ();
+
+  a_add = (fun x y r s ->
+    let open FStar.UInt8 in
+    assert (exists x'. r == Real.of_int x' /\ v x == x' % 256);
+    assert (exists y'. s == Real.of_int y' /\ v y == y' % 256);
+    let x' = FStar.IndefiniteDescription.indefinite_description_ghost int (fun x' -> r == Real.of_int x' /\ v x == x' % 256) in
+    let y' = FStar.IndefiniteDescription.indefinite_description_ghost int (fun y' -> s == Real.of_int y' /\ v y == y' % 256) in
+    let z' = x' + y' in
+    assert (r +. s == Real.of_int z');
+    ()
+  );
+
+  a_mul = (fun x y r s ->
+    let open FStar.UInt8 in
+    assert (exists x'. r == Real.of_int x' /\ v x == x' % 256);
+    assert (exists y'. s == Real.of_int y' /\ v y == y' % 256);
+    let x' = FStar.IndefiniteDescription.indefinite_description_ghost int (fun x' -> r == Real.of_int x' /\ v x == x' % 256) in
+    let y' = FStar.IndefiniteDescription.indefinite_description_ghost int (fun y' -> s == Real.of_int y' /\ v y == y' % 256) in
+    let z' = x' * y' in
+    mod_prod x' y' 256;
+    assert (z' % 256 == UInt8.v (x *%^ y));
+    assert (r *. s == Real.of_int z');
+    ()
+  );
+}
