src/lib/kuiper/Kuiper.Approximates.fsti
@@ -1,50 +1,19 @@
 module Kuiper.Approximates
 
+include Kuiper.Approximates.Class
+
+include Kuiper.Approximates.U8
+include Kuiper.Approximates.U16
+include Kuiper.Approximates.U32
+include Kuiper.Approximates.U64
+include Kuiper.Approximates.F16
+include Kuiper.Approximates.F32
+include Kuiper.Approximates.F64
+
 open Kuiper
 open FStar.Real
 open Kuiper.Scalars
 open Kuiper.Seq.Common
-
-class real_like (a:Type) {| scalar a |} = {
-  to_real : a -> real;
-
-  approximates : a -> real -> prop;
-
-  to_real_ok :
-    x:a ->
-    Lemma (ensures x `approximates` to_real x)
-          [SMTPat (x `approximates` to_real x)];
-
-  (* We assume these two values exist and approximate correctly *)
-
-  a0 : squash (approximates zero 0.0R);
-  a1 : squash (approximates one 1.0R);
-
-  a_add : x:a -> y:a -> r:real -> s:real ->
-          Lemma (requires approximates x r /\ approximates y s)
-                (ensures approximates (x `add` y) (r +. s))
-                [SMTPat (approximates x r); SMTPat (approximates y s)];
-                // ^ Does not kick in
-
-  a_mul : x:a -> y:a -> r:real -> s:real ->
-          Lemma (requires approximates x r /\ approximates y s)
-                (ensures approximates (x `mul` y) (r *. s))
-                [SMTPat (approximates x r); SMTPat (approximates y s)];
-                // ^ Does not kick in
-}
-
-(* We assume these types approximate reals *)
-instance val real_like_f16 : real_like f16
-instance val real_like_f32 : real_like f32
-instance val real_like_f64 : real_like f64
-
-(* For the integer types, we can actually define the relation
-and prove it. BUT, we must consider overflow! So we make the relation
-weaker than you may expect. *)
-instance val real_like_u8 : real_like u8
-instance val real_like_u16 : real_like u16
-instance val real_like_u32 : real_like u32
-instance val real_like_u64 : real_like u64
 
 let seq_approximates (#a:Type) {| scalar a, real_like a |}
   (s : seq a) (r : seq Real.real) : prop
